Prove S4 is sound

coq/Modal_Library.v
@@ -352,6 +352,9 @@ Definition conversely_well_founded_frame: Prop :=
 Definition noetherian_frame: Prop :=
   transitive_frame /\ conversely_well_founded_frame.
 
+Definition equivalence_frame: Prop :=
+  reflexivity_frame /\ transitivity_frame.
+
 End Classes.
 
 (* Logical Equivalence *)
